Weidenbach_Book/IsaSAT_Restart_LLVM.thy
@@ -2,153 +2,6 @@ theory IsaSAT_Restart_LLVM
   imports IsaSAT_Restart IsaSAT_Restart_Heuristics_LLVM IsaSAT_CDCL_LLVM
 begin
 
-sepref_register length_avdom
-
-sepref_register clause_is_learned_heur
-
-(*TODO Move: replace other verision*)
-lemma length_avdom_alt_def:
-  \<open>length_avdom = (\<lambda>(M', N', D', j, W', vm, \<phi>, clvls, cach, lbd, outl, stats, heur, vdom, avdom, lcount). length avdom)\<close>
-  by (intro ext) (auto simp: length_avdom_def)
-
-lemma get_the_propagation_reason_heur_alt_def:
-  \<open>get_the_propagation_reason_heur = (\<lambda>(M', N', D', j, W', vm, \<phi>, clvls, cach, lbd, outl, stats, heur, vdom, lcount) L .
-    get_the_propagation_reason_pol M' L)\<close>
-  by (intro ext) (auto simp: get_the_propagation_reason_heur_def)
-
-(*END Move*)
-
-sepref_def length_avdom_fast_code
-  is \<open>RETURN o length_avdom\<close>
-  :: \<open>isasat_bounded_assn\<^sup>k \<rightarrow>\<^sub>a sint64_nat_assn\<close>
-  unfolding length_avdom_alt_def access_vdom_at_pre_def isasat_bounded_assn_def
-  supply [[goals_limit = 1]]
-  by sepref
-
-sepref_register get_the_propagation_reason_heur
-
-sepref_def get_the_propagation_reason_heur_fast_code
-  is \<open>uncurry get_the_propagation_reason_heur\<close>
-  :: \<open>isasat_bounded_assn\<^sup>k *\<^sub>a unat_lit_assn\<^sup>k \<rightarrow>\<^sub>a snat_option_assn' TYPE(64)\<close>
-  unfolding get_the_propagation_reason_heur_alt_def access_vdom_at_pre_def
-     isasat_bounded_assn_def
-  supply [[goals_limit = 1]]
-  by sepref
-
-(*TODO Move: rplace*)
-
-lemma clause_is_learned_heur_alt_def:
-  \<open>clause_is_learned_heur = (\<lambda>(M', N', D', j, W', vm, \<phi>, clvls, cach, lbd, outl, stats, heur,
-    vdom, lcount) C . arena_status N' C = LEARNED)\<close>
-  by (intro ext) (auto simp: clause_is_learned_heur_def)
-(*ENED Move*)
-
-sepref_def clause_is_learned_heur_code2
-  is \<open>uncurry (RETURN oo clause_is_learned_heur)\<close>
-  :: \<open>[\<lambda>(S, C). arena_is_valid_clause_vdom (get_clauses_wl_heur S) C]\<^sub>a
-      isasat_bounded_assn\<^sup>k *\<^sub>a sint64_nat_assn\<^sup>k \<rightarrow> bool1_assn\<close>
-  supply [[goals_limit = 1]]
-  unfolding clause_is_learned_heur_alt_def isasat_bounded_assn_def
-  by sepref
-
-sepref_register clause_lbd_heur
-
-
-lemma clause_lbd_heur_alt_def:
-  \<open>clause_lbd_heur = (\<lambda>(M', N', D', j, W', vm, \<phi>, clvls, cach, lbd, outl, stats, heur, vdom, lcount) C.
-     arena_lbd N' C)\<close>
-  by (intro ext) (auto simp: clause_lbd_heur_def)
-
-sepref_def clause_lbd_heur_code2
-  is \<open>uncurry (RETURN oo clause_lbd_heur)\<close>
-  :: \<open>[\<lambda>(S, C). get_clause_LBD_pre (get_clauses_wl_heur S) C]\<^sub>a
-       isasat_bounded_assn\<^sup>k *\<^sub>a sint64_nat_assn\<^sup>k \<rightarrow> uint32_nat_assn\<close>
-  unfolding isasat_bounded_assn_def clause_lbd_heur_alt_def
-  supply [[goals_limit = 1]]
-  by sepref
-
-sepref_register mark_garbage_heur
-
-
-sepref_def mark_garbage_heur_code2
-  is \<open>uncurry2 (RETURN ooo mark_garbage_heur)\<close>
-  :: \<open>[\<lambda>((C, i), S). mark_garbage_pre (get_clauses_wl_heur S, C) \<and> i < length_avdom S \<and>
-         get_learned_count S \<ge> 1]\<^sub>a
-       sint64_nat_assn\<^sup>k *\<^sub>a sint64_nat_assn\<^sup>k *\<^sub>a isasat_bounded_assn\<^sup>d \<rightarrow> isasat_bounded_assn\<close>
-  supply [[goals_limit = 1]]
-  unfolding mark_garbage_heur_def isasat_bounded_assn_def delete_index_and_swap_alt_def
-    length_avdom_def fold_tuple_optimizations
-  apply (annot_unat_const "TYPE(64)")
-  by sepref
-
-sepref_register delete_index_vdom_heur
-
-
-sepref_def delete_index_vdom_heur_fast_code2
-  is \<open>uncurry (RETURN oo delete_index_vdom_heur)\<close>
-  :: \<open>[\<lambda>(i, S). i < length_avdom S]\<^sub>a
-        sint64_nat_assn\<^sup>k *\<^sub>a isasat_bounded_assn\<^sup>d \<rightarrow> isasat_bounded_assn\<close>
-  supply [[goals_limit = 1]]
-  unfolding delete_index_vdom_heur_def isasat_bounded_assn_def delete_index_and_swap_alt_def
-    length_avdom_def fold_tuple_optimizations
-  by sepref
-
-sepref_register access_length_heur
-
-sepref_def access_length_heur_fast_code2
-  is \<open>uncurry (RETURN oo access_length_heur)\<close>
-  :: \<open>[\<lambda>(S, C). arena_is_valid_clause_idx (get_clauses_wl_heur S) C]\<^sub>a
-       isasat_bounded_assn\<^sup>k *\<^sub>a sint64_nat_assn\<^sup>k \<rightarrow> sint64_nat_assn\<close>
-  supply [[goals_limit = 1]]
-  unfolding access_length_heur_alt_def isasat_bounded_assn_def fold_tuple_optimizations
-  by sepref
-
-sepref_register marked_as_used_st
-
-sepref_def marked_as_used_st_fast_code
-  is \<open>uncurry (RETURN oo marked_as_used_st)\<close>
-  :: \<open>[\<lambda>(S, C). marked_as_used_pre (get_clauses_wl_heur S) C]\<^sub>a
-       isasat_bounded_assn\<^sup>k *\<^sub>a sint64_nat_assn\<^sup>k \<rightarrow> bool1_assn\<close>
-  supply [[goals_limit = 1]]
-  unfolding marked_as_used_st_alt_def isasat_bounded_assn_def fold_tuple_optimizations
-  by sepref
-
-lemma arena_act_pre_mark_used:
-  \<open>arena_act_pre arena C \<Longrightarrow>
-  arena_act_pre (mark_unused arena C) C\<close>
-  unfolding arena_act_pre_def arena_is_valid_clause_idx_def
-  apply clarify
-  apply (rule_tac x=N in exI)
-  apply (rule_tac x=vdom in exI)
-  by (auto simp: arena_act_pre_def
-    simp: valid_arena_mark_unused)
-
-
-sepref_register mark_unused_st_heur
-sepref_def mark_unused_st_fast_code
-  is \<open>uncurry (RETURN oo mark_unused_st_heur)\<close>
-  :: \<open>[\<lambda>(C, S). arena_act_pre (get_clauses_wl_heur S) C]\<^sub>a
-        sint64_nat_assn\<^sup>k *\<^sub>a isasat_bounded_assn\<^sup>d \<rightarrow> isasat_bounded_assn\<close>
-  unfolding mark_unused_st_heur_def isasat_bounded_assn_def
-    arena_act_pre_mark_used[intro!]
-  supply [[goals_limit = 1]]
-  by sepref
-
-sepref_register mark_clauses_as_unused_wl_D_heur
-
-declare clause_not_marked_to_delete_heur_fast_code.refine[sepref_fr_rules]
-
-sepref_def mark_clauses_as_unused_wl_D_heur_fast_code
-  is \<open>uncurry mark_clauses_as_unused_wl_D_heur\<close>
-  :: \<open>[\<lambda>(_, S). length (get_avdom S) \<le> sint64_max]\<^sub>a
-    sint64_nat_assn\<^sup>k *\<^sub>a isasat_bounded_assn\<^sup>d \<rightarrow> isasat_bounded_assn\<close>
-  supply [[goals_limit=1]] length_avdom_def[simp]
-  unfolding mark_clauses_as_unused_wl_D_heur_def
-    mark_unused_st_heur_def[symmetric]
-    access_vdom_at_def[symmetric] length_avdom_def[symmetric]
-  apply (annot_snat_const "TYPE(64)")
-  by sepref
-
 
 sepref_register mark_to_delete_clauses_wl_D_heur
 
@@ -176,17 +29,6 @@ sepref_def mop_clause_not_marked_to_delete_heur_impl
   by sepref
 
 
-lemma mop_mark_garbage_heur_alt_def:
-  \<open>mop_mark_garbage_heur C i = (\<lambda>(M', N', D', j, W', vm, \<phi>, clvls, cach, lbd, outl, stats, heur,
-       vdom, avdom, lcount, opts, old_arena). do {
-    ASSERT(mark_garbage_pre (get_clauses_wl_heur (M', N', D', j, W', vm, \<phi>, clvls, cach, lbd, outl, stats, heur,
-       vdom, avdom, lcount, opts, old_arena), C) \<and> lcount \<ge> 1 \<and> i < length avdom);
-    RETURN (M', extra_information_mark_to_delete N' C, D', j, W', vm, \<phi>, clvls, cach, lbd, outl, stats,
-      heur,
-       vdom, delete_index_and_swap avdom i, lcount - 1, opts, old_arena)
-   })\<close>
-  unfolding mop_mark_garbage_heur_def mark_garbage_heur_def
-  by (auto intro!: ext)
 
 
 sepref_def delete_index_and_swap_code2
@@ -296,7 +138,7 @@ sepref_def mop_arena_length_st_impl
   unfolding mop_arena_length_st_alt_def isasat_bounded_assn_def
   by sepref
 (*END Move*)
-find_theorems name:arena_length name:st
+
 sepref_def mark_to_delete_clauses_wl_D_heur_fast_impl
   is \<open>mark_to_delete_clauses_wl_D_heur\<close>
   :: \<open>[\<lambda>S. length (get_clauses_wl_heur S) \<le> sint64_max]\<^sub>a isasat_bounded_assn\<^sup>d \<rightarrow> isasat_bounded_assn\<close>
